compiler/bootstrap/translation/arm6ProgScript.sml
@@ -1,15 +1,13 @@
 open preamble;
 open terminationTheory
 open ml_translatorLib ml_translatorTheory;
-open compiler32ProgTheory
+open to_target32ProgTheory
 open arm6_targetTheory armTheory;
 open inliningLib;
 
 val _ = new_theory "arm6Prog"
 
-val _ = translation_extends "compiler32Prog";
-
-val RW = REWRITE_RULE
+val _ = translation_extends "to_target32Prog";
 
 val _ = add_preferred_thy "-";
 val _ = add_preferred_thy "termination";
@@ -33,7 +31,7 @@ fun def_of_const tm = let
   val def = def_from_thy "termination" name handle HOL_ERR _ =>
             def_from_thy (#Thy res) name handle HOL_ERR _ =>
             failwith ("Unable to find definition of " ^ name)
-  val def = def |> RW (!extra_preprocessing)
+  val def = def |> REWRITE_RULE (!extra_preprocessing)
                 |> CONV_RULE (DEPTH_CONV BETA_CONV)
                 (* TODO: This ss messes up defs containing if-then-else
                 with constant branches
@@ -42,28 +40,6 @@ fun def_of_const tm = let
   in def end
 
 val _ = (find_def_for_const := def_of_const);
-
-val spec32 = INST_TYPE[alpha|->``:32``]
-
-val conv32_RHS = GEN_ALL o CONV_RULE (RHS_CONV wordsLib.WORD_CONV) o spec32 o SPEC_ALL
-
-val word_bit_thm = Q.prove(
-  `!n w. word_bit n w = ((w && n2w (2 ** n)) <> 0w)`,
-  simp [GSYM wordsTheory.word_1_lsl]
-  \\ srw_tac [wordsLib.WORD_BIT_EQ_ss] [wordsTheory.word_index]
-  \\ eq_tac
-  \\ rw []
-  >- (qexists_tac `n` \\ simp [DECIDE ``0 < a /\ n <= a - 1n ==> n < a``])
-  \\ `i = n` by decide_tac
-  \\ fs [])
-
-(* word_concat *)
-val wc_simp = CONV_RULE (wordsLib.WORD_CONV) o SIMP_RULE std_ss [word_concat_def,word_join_def,w2w_w2w,LET_THM]
-(* word_extract *)
-val we_simp = SIMP_RULE std_ss [word_extract_w2w_mask,w2w_id]
-
-val gconv = CONV_RULE (DEPTH_CONV wordsLib.WORD_GROUND_CONV)
-val econv = CONV_RULE wordsLib.WORD_EVAL_CONV
 
 val v2w_rw = Q.prove(`
   v2w [P] = if P then 1w else 0w`,
@@ -219,12 +195,6 @@ val arm6_enc36 = replace_at 36 (fn th => th |> SIMP_RULE (srw_ss()) [WORD_LO,wor
 |> finish |> SIMP_RULE (srw_ss())[word_2comp_def])
 
 val arm6_enc_thm = List.tabulate (36, fn i => Array.sub(arm6_enc_thms,i)) |> LIST_CONJ
-
-(* the manual translation of w2w should no longer be necessary
-val w2ws = mk_set(map type_of ((find_terms (fn t => same_const ``w2w`` t)) (concl arm6_enc_thm)))
-
-val res = map (fn ty => let val (l,r) = dom_rng ty in INST_TYPE[alpha|->wordsSyntax.dest_word_type l,beta|->wordsSyntax.dest_word_type r] w2w_def |> translate end) w2ws;
-*)
 
 val _ = translate (EncodeARMImmediate_def |> SIMP_RULE (srw_ss()) [Ntimes EncodeARMImmediate_aux_def 16] |> finish |> SIMP_RULE (srw_ss()) [word_2comp_def])
 
